Add unfold to fix examples (cf Nik) + fix proofs

iodiv/Tests.fst
@@ -31,11 +31,7 @@ let test (s : string) : IODiv unit (requires True) (ensures fun _ -> True) =
   close fd
 
 let test_ (s : string) : IODiv unit (requires True) (ensures fun r -> terminates r /\ (exists fd msg. ret_trace r == [ EOpenfile s fd ; ERead fd msg ; EClose fd () ]))
-by (
-  explode ()
-)
-=
-  let fd = open_file s in
+= let fd = open_file s in
   let msg = read fd in
   close fd
 
@@ -45,16 +41,6 @@ let test'' (fd : file_descr) : IODiv unit (requires True) (ensures fun _ -> True
 
 let test_more (fd : file_descr) : IODiv unit (requires True) (ensures fun _ -> True) =
   test'' fd ; test'' fd
-
-// let test_more' (fd : file_descr) : IODiv unit (requires True) (ensures fun _ -> True) =
-//   // assume (forall (w1 w2 : twp unit). w1 `stronger_twp` w2) ;
-//   // assume (forall (w : twp unit). (fun p -> True /\ (forall x. (fun _ -> True) x ==> p x)) `stronger_twp` w) ;
-//   // assume (forall (w : twp unit) (wf : unit -> twp unit). (fun p -> True /\ (forall x. (fun _ -> True) x ==> p x)) `stronger_twp` wbind w wf) ;
-//   assume (forall (wf : unit -> twp unit). (fun p -> True /\ (forall x. (fun _ -> True) x ==> p x)) `stronger_twp` wbind (fun p -> True /\ (forall x. (fun _ -> True) x ==> p x)) wf) ; // Enough, note it's wbind and not pwbind
-//   // assume ((fun p -> True /\ (forall x. (fun _ -> True) x ==> p x)) `stronger_twp` wbind #unit #unit (fun p -> True /\ (forall x. (fun _ -> True) x ==> p x)) (fun (x : unit) -> (fun p -> True /\ (forall x. (fun _ -> True) x ==> p x)))) ; // Not that one
-//   test'' fd ;
-//   test'' fd ;
-//   test'' fd
 
 let test_more' (fd : file_descr) : IODiv unit (requires True) (ensures fun _ -> True) =
   test'' fd ;
@@ -66,9 +52,6 @@ let test3 (fd : file_descr) : IODiv unit (requires True) (ensures fun _ -> True)
   () ; () ; ()
 
 let test' (s : string) : IODiv unit (requires True) (ensures fun _ -> True)
-by (
-  explode ()
-)
 = let fd = open_file s in
   let msg = read fd in
   ()
@@ -81,23 +64,14 @@ let open_close_test (s : string) : IODiv unit (requires True) (ensures fun r -> 
   let fd = open_file s in
   close fd
 
-// let many_open_test (s : string) : IODiv unit (requires True) (ensures fun r -> terminates r)
-// by (
-//   explode () ;
-//   bump_nth 5 ;
-//   squash_intro () ;
-//   dump "hhop"
-// )
-// = let x = open_file s in
-//   let y = open_file s in
-//   ()
+let many_open_test (s : string) : IODiv unit (requires True) (ensures fun r -> terminates r)
+= let x = open_file s in
+  let y = open_file s in
+  ()
 
 let many_open_test' (s : string) : IODiv file_descr (requires True) (ensures fun r -> terminates r) =
   let x = open_file s in
   open_file s
-
-// From this, it seems every time I stack more than two binds I get an error.
-// But () ; () is ok.
 
 // Fails because it can't infer something (the w??)
 // let repeat_open_close_test (s : string) : IODiv unit (requires True) (ensures fun _ -> True) =
